<?xml version="1.0" encoding="utf-8"?>
<rdf:RDF
  xmlns:owl="http://www.w3.org/2002/07/owl#"
  xmlns:rdf="http://www.w3.org/1999/02/22-rdf-syntax-ns#"
  xmlns:schema="https://schema.org/"
  xmlns:dcterms="http://purl.org/dc/terms/"
  xmlns:rdfs="http://www.w3.org/2000/01/rdf-schema#"
  
>

	<!-- §7.1  EarthObservation -->

  <rdfs:Class rdf:about="https://schema.org/EarthObservation">
    <owl:equivalentClass rdf:resource="http://www.opengis.net/ont/eo-geojson/1.0/EarthObservation"/>
    <dcterms:source rdf:resource="http://docs.opengeospatial.org/is/17-003r2/17-003r2.html"/>
    <rdfs:label>EarthObservation</rdfs:label>
    <rdfs:subClassOf rdf:resource="https://schema.org/Dataset"/>
    <rdfs:comment>Earth Observation granule or product as defined in OGC 10-157r4 and OGC 17-003r2.</rdfs:comment>
  </rdfs:Class>
   
  
	<!-- §7.1  Properties -->
  
  
   <rdf:Property rdf:about="https://schema.org/acquisitionInformation">
    <schema:rangeIncludes rdf:resource="https://schema.org/AcquisitionInformation"/>
    <schema:isPartOf rdf:resource="http://eo.schema.org"/>
    <rdfs:comment>Acquisition information related to the dataset.</rdfs:comment>
    <rdfs:label>acquisitionInformation</rdfs:label>
    <schema:domainIncludes rdf:resource="https://schema.org/EarthObservation"/>
    <owl:equivalentProperty rdf:resource="http://www.opengis.net/ont/eo-geojson/1.0/acquisitionInformation"/>
    <dcterms:source rdf:resource="http://docs.opengeospatial.org/is/17-003r2/17-003r2.html#44"/>
  </rdf:Property>
  
    <rdf:Property rdf:about="https://schema.org/productInformation">
    <dcterms:source rdf:resource="http://docs.opengeospatial.org/is/17-003r2/17-003r2.html"/>
    <schema:domainIncludes rdf:resource="https://schema.org/EarthObservation"/>
    <rdfs:comment>Product information related to the dataset.</rdfs:comment>
    <owl:equivalentProperty rdf:resource="http://www.opengis.net/ont/eo-geojson/1.0/productInformation"/>
    <schema:isPartOf rdf:resource="http://eo.schema.org"/>
    <rdfs:label>productInformation</rdfs:label>
    <schema:rangeIncludes rdf:resource="https://schema.org/ProductInformation"/>
  </rdf:Property>
  
  <rdf:Property rdf:about="https://schema.org/acquisitionStatus">
    <schema:domainIncludes rdf:resource="https://schema.org/EarthObservation"/>
    <rdfs:label>acquisitionStatus</rdfs:label>
    <schema:isPartOf rdf:resource="http://eo.schema.org"/>
    <schema:rangeIncludes rdf:resource="https://schema.org/AcquisitionStatusType"/>
    <dcterms:source rdf:resource="http://docs.opengeospatial.org/is/17-003r2/17-003r2.html"/>
    <owl:equivalentProperty rdf:resource="http://www.opengis.net/ont/eo-geojson/1.0/status"/>
    <rdfs:comment>Refers to product status.

Fixed Values :
 - ARCHIVED
 - ACQUIRED
 - CANCELLED
 - FAILED
 - PLANNED
 - POTENTIAL
 - REJECTED
 - QUALITYDEGRADED.</rdfs:comment>
  </rdf:Property>
    
  <rdfs:Class rdf:about="https://schema.org/AcquisitionStatusType">
    <owl:equivalentClass rdf:resource="http://www.opengis.net/ont/eo-geojson/1.0/statusType"/>
    <schema:isPartOf rdf:resource="http://eo.schema.org"/>
    <rdfs:comment>Enumeration of acquisition status constants.</rdfs:comment>
    <rdfs:subClassOf rdf:resource="https://schema.org/Enumeration"/>
    <rdfs:label>AcquisitionStatusType</rdfs:label>
  </rdfs:Class>
  
  
  <schema:AcquisitionStatusType rdf:about="https://schema.org/ARCHIVED">
    <rdfs:comment>Acquisition status constant.</rdfs:comment>
    <rdfs:label>ARCHIVED</rdfs:label>
  </schema:AcquisitionStatusType>
  
  <schema:AcquisitionStatusType rdf:about="https://schema.org/ACQUIRED">
    <rdfs:comment>Acquisition status constant.</rdfs:comment>
    <rdfs:label>ACQUIRED</rdfs:label>
  </schema:AcquisitionStatusType>
  
   <schema:AcquisitionStatusType rdf:about="https://schema.org/POTENTIAL">
    <rdfs:comment>Acquisition status constant.</rdfs:comment>
    <rdfs:label>POTENTIAL</rdfs:label>
  </schema:AcquisitionStatusType>
  
  <schema:AcquisitionStatusType rdf:about="https://schema.org/CANCELLED">
    <rdfs:comment>Acquisition status constant.</rdfs:comment>
    <rdfs:label>CANCELLED</rdfs:label>
  </schema:AcquisitionStatusType>
  
  <schema:AcquisitionStatusType rdf:about="https://schema.org/FAILED">
    <rdfs:label>FAILED</rdfs:label>
    <rdfs:comment>Acquisition status constant.</rdfs:comment>
  </schema:AcquisitionStatusType>
  
   <schema:AcquisitionStatusType rdf:about="https://schema.org/REJECTED">
    <rdfs:label>REJECTED</rdfs:label>
    <rdfs:comment>Acquisition status constant.</rdfs:comment>
  </schema:AcquisitionStatusType>
  
   <schema:AcquisitionStatusType rdf:about="https://schema.org/PLANNED">
    <rdfs:label>PLANNED</rdfs:label>
    <rdfs:comment>Acquisition status constant.</rdfs:comment>
  </schema:AcquisitionStatusType>
  
    
  <schema:AcquisitionStatusType rdf:about="https://schema.org/QUALITYDEGRADED">
    <rdfs:label>QUALITYDEGRADED</rdfs:label>
    <rdfs:comment>Acquisition status constant.</rdfs:comment>
  </schema:AcquisitionStatusType>
  
  
  
  <!-- §7.3  DataIdentification  -->
  
  <rdf:Property rdf:about="https://schema.org/parentIdentifier">
    <schema:rangeIncludes rdf:resource="https://schema.org/Text"/>
    <schema:rangeIncludes rdf:resource="https://schema.org/URL"/>  
    <!-- added 05/07/2021 -->
    <rdfs:subPropertyOf rdf:resource="https://schema.org/isPartOf"/>    
    <schema:isPartOf rdf:resource="http://eo.schema.org"/>
    <dcterms:source rdf:resource="http://docs.opengeospatial.org/is/17-003r2/17-003r2.html"/>
    <schema:domainIncludes rdf:resource="https://schema.org/EarthObservation"/>
    <rdfs:comment>Collection the granule belongs to.</rdfs:comment>
    <rdfs:label>parentIdentifier</rdfs:label>
  </rdf:Property>
  
  
  <!-- added 05/07/2021 -->
  <rdf:Property rdf:about="https://schema.org/available">
    <rdfs:label>available</rdfs:label>
    <schema:rangeIncludes rdf:resource="https://schema.org/DateTime"/>
    <schema:rangeIncludes rdf:resource="https://schema.org/Text"/>
    <rdfs:comment>Date range during which the resource will be available ISO 8601.</rdfs:comment>
    <schema:domainIncludes rdf:resource="https://schema.org/EarthObservation"/>
    <dcterms:source rdf:resource="http://docs.opengeospatial.org/is/17-003r2/17-003r2.html"/>
     <owl:equivalentProperty rdf:resource="http://purl.org/dc/terms/available"/>
  </rdf:Property>
  
  
   <!-- §7.4.2  VerticalSpatialDomain  -->
  
   <rdfs:Class rdf:about="https://schema.org/VerticalSpatialDomain">
    <rdfs:comment>Contains the properties related to the spatial extent in the vertical dimension.  Its properties are inherited by the AcquisitionParameters object. 
  UnitText used to express minValue (lowestLocation) and maxValue (highestLocation) should be meter (m) or bar (bar). Default is meter (m).</rdfs:comment>
    <rdfs:subClassOf rdf:resource="https://schema.org/QuantitativeValue"/>
    <rdfs:subClassOf rdf:resource="https://schema.org/VirtualLocation"/>  <!-- can be in range of location property -->
    <owl:equivalentClass rdf:resource="http://www.opengis.net/ont/eo-geojson/1.0/VerticalSpatialDomain"/>
    <schema:isPartOf rdf:resource="http://eo.schema.org"/>
    <dcterms:source rdf:resource="http://docs.opengeospatial.org/is/17-003r2/17-003r2.html"/>
    <rdfs:label>VerticalSpatialDomain</rdfs:label>
  </rdfs:Class>
    
  
   <!-- §7.4.3  OrbitParameters  -->
   
  <rdfs:Class rdf:about="https://schema.org/OrbitParameters">
    <rdfs:subClassOf rdf:resource="https://schema.org/StructuredValue"/>
    <rdfs:label>OrbitParameters</rdfs:label>
    <dcterms:source rdf:resource="http://docs.opengeospatial.org/is/17-003r2/17-003r2.html"/>
    <owl:equivalentClass rdf:resource="http://www.opengis.net/ont/eo-geojson/1.0/OrbitParameters"/>
    <schema:isPartOf rdf:resource="http://eo.schema.org"/>
    <rdfs:comment>Contains the properties related to the orbit.  Its properties are inherited by the AcquisitionParameters object.</rdfs:comment>
  </rdfs:Class>
  
  <rdf:Property rdf:about="https://schema.org/orbitDirection">
    <owl:equivalentProperty rdf:resource="http://www.opengis.net/ont/eo-geojson/1.0/orbitDirection"/>
    <rdfs:comment>Product information related to the dataset.</rdfs:comment>
    <rdfs:comment>Acquisition orbit direction at the start of the acquisition/product.
Values:
•	ASCENDING
•	DESCENDING</rdfs:comment>
    <dcterms:source rdf:resource="http://docs.opengeospatial.org/is/17-003r2/17-003r2.html"/>
    <schema:rangeIncludes rdf:resource="https://schema.org/OrbitDirectionType"/>
    <schema:domainIncludes rdf:resource="https://schema.org/OrbitParameters"/>
    <rdfs:label>orbitDirection</rdfs:label>
    <schema:isPartOf rdf:resource="http://eo.schema.org"/>
  </rdf:Property>
  
  
   <rdfs:Class rdf:about="https://schema.org/OrbitDirectionType">
    <rdfs:comment>Enumeration of orbit direction constants.</rdfs:comment>
    <rdfs:label>OrbitDirectionType</rdfs:label>
    <rdfs:subClassOf rdf:resource="https://schema.org/Enumeration"/>
    <owl:equivalentClass rdf:resource="http://www.opengis.net/ont/eo-geojson/1.0/OrbitDirectionType"/>
    <schema:isPartOf rdf:resource="http://eo.schema.org"/>
  </rdfs:Class>
  
  
   <schema:OrbitDirectionType rdf:about="https://schema.org/ASCENDING">
    <rdfs:label>ASCENDING</rdfs:label>
    <rdfs:comment>Orbit direction constant.</rdfs:comment>
  </schema:OrbitDirectionType>
  
   <schema:OrbitDirectionType rdf:about="https://schema.org/DESCENDING">
    <rdfs:comment>Orbit direction constant.</rdfs:comment>
    <rdfs:label>DESCENDING</rdfs:label>
  </schema:OrbitDirectionType>
  
  
   <rdf:Property rdf:about="https://schema.org/lastOrbitDirection">
    <rdfs:comment>Acquisition orbit direction at the end of the acquisition/product. Assumed to be identical to orbitDirection if not present.
Values:
•	ASCENDING
•	DESCENDING</rdfs:comment>
    <rdfs:label>lastOrbitDirection</rdfs:label>
    <schema:domainIncludes rdf:resource="https://schema.org/OrbitParameters"/>
    <schema:rangeIncludes rdf:resource="https://schema.org/OrbitDirectionType"/>
    <dcterms:source rdf:resource="http://docs.opengeospatial.org/is/17-003r2/17-003r2.html"/>
  </rdf:Property>
  
  <rdf:Property rdf:about="https://schema.org/orbitDuration">
    <rdfs:comment>Actual orbit duration in ISO 8601 duration format (range is TBD).</rdfs:comment>
    <dcterms:source rdf:resource="http://docs.opengeospatial.org/is/17-003r2/17-003r2.html"/>
    <schema:domainIncludes rdf:resource="https://schema.org/OrbitParameters"/>
    <rdfs:subPropertyOf rdf:resource="https://schema.org/duration"/>
    <rdfs:label>orbitDuration</rdfs:label>
    <schema:rangeIncludes rdf:resource="https://schema.org/Duration"/>
  </rdf:Property>
  
 
  
  <rdf:Property rdf:about="https://schema.org/orbitNumber">
    <schema:domainIncludes rdf:resource="https://schema.org/OrbitParameters"/>
    <dcterms:source rdf:resource="http://docs.opengeospatial.org/is/17-003r2/17-003r2.html"/>
    <rdfs:label>orbitNumber</rdfs:label>
    <rdfs:comment>Acquisition orbit number.</rdfs:comment>
    <schema:rangeIncludes rdf:resource="https://schema.org/Integer"/>
  </rdf:Property>
  
  <rdf:Property rdf:about="https://schema.org/lastOrbitNumber">
    <schema:domainIncludes rdf:resource="https://schema.org/OrbitParameters"/>
    <rdfs:label>lastOrbitNumber</rdfs:label>
    <schema:rangeIncludes rdf:resource="https://schema.org/Integer"/>
    <rdfs:comment>Acquisition last orbit number.</rdfs:comment>
    <dcterms:source rdf:resource="http://docs.opengeospatial.org/is/17-003r2/17-003r2.html"/>
  </rdf:Property>
  
   <rdf:Property rdf:about="https://schema.org/ascendingNodeDate">
    <dcterms:source rdf:resource="http://docs.opengeospatial.org/is/17-003r2/17-003r2.html"/>
    <schema:rangeIncludes rdf:resource="https://schema.org/DateTime"/>
    <rdfs:label>ascendingNodeDate</rdfs:label>
    <schema:domainIncludes rdf:resource="https://schema.org/OrbitParameters"/>
    <rdfs:comment>UTC date and time at ascending node of orbit.</rdfs:comment>
  </rdf:Property>
  
  <rdf:Property rdf:about="https://schema.org/ascendingNodeLongitude">
    <rdfs:subPropertyOf rdf:resource="https://schema.org/longitude"/>
    <schema:rangeIncludes rdf:resource="https://schema.org/Number"/>
    <schema:rangeIncludes rdf:resource="https://schema.org/Text"/>
    <rdfs:label>ascendingNodeLongitude</rdfs:label>
    <rdfs:comment>Longitude at ascending node of orbit. Should be expressed in degrees.</rdfs:comment>
    <dcterms:source rdf:resource="http://docs.opengeospatial.org/is/17-003r2/17-003r2.html"/>
    <schema:domainIncludes rdf:resource="https://schema.org/OrbitParameters"/>
  </rdf:Property>
  
  
  
   <!-- §7.5  Temporal Information  -->
   
   <!-- Covered by existing properties. -->
   
   <!-- §7.6  AcquisitionInformation  -->
   
   <rdfs:Class rdf:about="https://schema.org/AcquisitionInformation">
    <dcterms:source rdf:resource="http://docs.opengeospatial.org/is/17-003r2/17-003r2.html#44"/>
    <owl:equivalentClass rdf:resource="http://www.opengis.net/ont/eo-geojson/1.0/AcquisitionInformation"/>
    <rdfs:label>AcquisitionInformation</rdfs:label>
    <dcterms:source rdf:resource="http://docs.opengeospatial.org/is/17-003r2/17-003r2.html"/>
    <rdfs:comment>Acquisition information of the Earth Observation as defined in OGC 17-003r2.</rdfs:comment>
    <rdfs:subClassOf rdf:resource="https://schema.org/StructuredValue"/>
  </rdfs:Class>
  
   
   <rdf:Property rdf:about="https://schema.org/platform">
    <schema:domainIncludes rdf:resource="https://schema.org/AcquisitionInformation"/>
    <schema:rangeIncludes rdf:resource="https://schema.org/Platform"/>
    <rdfs:label>platform</rdfs:label>
    <rdfs:comment>The Platform used for the acquisition.  If more than one platform is used for creating the product, then the AcquisitionInformation object occurs more than once.</rdfs:comment>
    <dcterms:source rdf:resource="http://docs.opengeospatial.org/is/17-003r2/17-003r2.html"/>
  </rdf:Property>
  
  <!-- 05/07/2021: renamed instrument as already defined in schema.org -->
  <rdf:Property rdf:about="https://schema.org/sensor">
    <dcterms:source rdf:resource="http://docs.opengeospatial.org/is/17-003r2/17-003r2.html"/>
    <rdfs:label>sensor</rdfs:label>
    <rdfs:comment>The Instrument/Sensor used for the acquisition.
If more than one instrument is used for creating the product, then the AcquisitionInformation object occurs more than once.</rdfs:comment>
    <schema:domainIncludes rdf:resource="https://schema.org/AcquisitionInformation"/>
    <schema:rangeIncludes rdf:resource="https://schema.org/Instrument"/>
  </rdf:Property>  
  
   <rdf:Property rdf:about="https://schema.org/acquisitionParameters">
    <schema:domainIncludes rdf:resource="https://schema.org/AcquisitionInformation"/>
    <dcterms:source rdf:resource="http://docs.opengeospatial.org/is/17-003r2/17-003r2.html"/>
    <rdfs:label>acquisitionParameters</rdfs:label>
    <rdfs:comment>The acquisition parameters (i.e. pointing angles, etc.).</rdfs:comment>
    <schema:rangeIncludes rdf:resource="https://schema.org/AcquisitionParameters"/>
  </rdf:Property>
  
  
   <!-- §7.6.1   Platform  -->
   
   <rdfs:Class rdf:about="https://schema.org/Platform">
    <rdfs:subClassOf rdf:resource="https://schema.org/Vehicle"/>
	<!--  <rdfs:subClassOf rdf:resource="https://schema.org/StructuredValue"/> -->
    <rdfs:seeAlso rdf:resource="https://gcmdservices.gsfc.nasa.gov/static/kms/platforms/platforms.rdf"/>
    <rdfs:label>Platform</rdfs:label>
    <rdfs:comment>Platform (satellite) that was used to perform the observation.  Use as "id" the URI defined by ESA or GCMD to identify the platform.</rdfs:comment>
    <dcterms:source rdf:resource="http://docs.opengeospatial.org/is/17-003r2/17-003r2.html"/>
  </rdfs:Class>
   
  <!-- platformShortName  -> schema:name (inherited) -->  
 
  <rdf:Property rdf:about="https://schema.org/serialNumber">
    <!-- platformSerialIdentifier  -->
    <schema:domainIncludes rdf:resource="https://schema.org/Platform"/>
  </rdf:Property>
      
  <rdf:Property rdf:about="https://schema.org/orbitType">
    <dcterms:source rdf:resource="http://docs.opengeospatial.org/is/17-003r2/17-003r2.html"/>
    <owl:equivalentProperty rdf:resource="http://www.opengis.net/ont/eo-geojson/1.0/orbitType"/>
    <schema:rangeIncludes rdf:resource="https://schema.org/OrbitType"/>
    <rdfs:comment>High level characterisation of main mission types taken from a codelist.</rdfs:comment>
    <schema:domainIncludes rdf:resource="https://schema.org/Platform"/>
    <rdfs:label>orbitType</rdfs:label>
  </rdf:Property>
  
   <rdfs:Class rdf:about="https://schema.org/OrbitType">
    <dcterms:source rdf:resource="http://docs.opengeospatial.org/is/17-003r2/17-003r2.html"/>
    <rdfs:subClassOf rdf:resource="https://schema.org/Enumeration"/>
    <rdfs:label>OrbitType</rdfs:label>
    <rdfs:comment>Enumeration of orbitType constants.</rdfs:comment>
  </rdfs:Class>
  
   <schema:OrbitType rdf:about="https://schema.org/LEO">
    <rdfs:label>LEO</rdfs:label>
    <rdfs:comment>Orbit type constant.</rdfs:comment>
  </schema:OrbitType>
  
  <schema:OrbitType rdf:about="https://schema.org/GEO">
    <rdfs:label>GEO</rdfs:label>
    <rdfs:comment>Orbit type constant.</rdfs:comment>
  </schema:OrbitType>
  
  
   <!-- §7.6.2   Instrument  -->
  
  
  <rdfs:Class rdf:about="https://schema.org/Instrument">
    <dcterms:source rdf:resource="http://docs.opengeospatial.org/is/17-003r2/17-003r2.html"/>
    <rdfs:label>Instrument</rdfs:label>
    <rdfs:subClassOf rdf:resource="https://schema.org/StructuredValue"/>
    <rdfs:comment>Contains the properties of the instrument that was used to perform the observation.  Use as "id" the URI defined by GCMD to identify the instrument.  A list of URI can be downloaded from https://gcmdservices.gsfc.nasa.gov/static/kms/instruments/instruments.rdf.</rdfs:comment>
  </rdfs:Class>
    
   <!-- instrumentShortName -> schema:name (inherited) -->
    
   <!-- decription -> schema:description (inherited) -->
  
     
   <rdf:Property rdf:about="https://schema.org/sensorType">
    <schema:rangeIncludes rdf:resource="https://schema.org/SensorType"/>
    <schema:domainIncludes rdf:resource="https://schema.org/Instrument"/>
    <rdfs:label>sensorType</rdfs:label>
    <dcterms:source rdf:resource="http://docs.opengeospatial.org/is/17-003r2/17-003r2.html"/>
    <rdfs:comment>Sensor type based on codelist.</rdfs:comment>
  </rdf:Property>
  
   <rdfs:Class rdf:about="https://schema.org/SensorType">
    <rdfs:subClassOf rdf:resource="https://schema.org/Enumeration"/>
    <rdfs:label>SensorType</rdfs:label>
    <dcterms:source rdf:resource="http://docs.opengeospatial.org/is/17-003r2/17-003r2.html"/>
    <rdfs:comment>Enumeration of sensorType constants.</rdfs:comment>
  </rdfs:Class>
  
  <schema:SensorType rdf:about="https://schema.org/OPTICAL">
    <rdfs:comment>Sensor type constant.</rdfs:comment>
    <rdfs:label>OPTICAL</rdfs:label>
  </schema:SensorType>
  
  <schema:SensorType rdf:about="https://schema.org/ATMOSPHERIC">
    <rdfs:comment>Sensor type constant.</rdfs:comment>
    <rdfs:label>ATMOSPHERIC</rdfs:label>
  </schema:SensorType>
  
  <schema:SensorType rdf:about="https://schema.org/ALTIMETRIC">
    <rdfs:comment>Sensor type constant.</rdfs:comment>
    <rdfs:label>ALTIMETRIC</rdfs:label>
  </schema:SensorType>
  
  <schema:SensorType rdf:about="https://schema.org/LIMB">
    <rdfs:comment>Sensor type constant.</rdfs:comment>
    <rdfs:label>LIMB</rdfs:label>
  </schema:SensorType>
  
  <schema:SensorType rdf:about="https://schema.org/RADAR">
    <rdfs:label>RADAR</rdfs:label>
    <rdfs:comment>Sensor type constant.</rdfs:comment>
  </schema:SensorType>
  
  
   <!-- §7.6.3   WavelengthInformation  -->
   
   <rdfs:Class rdf:about="https://schema.org/WavelengthInformation">
    <rdfs:label>WavelengthInformation</rdfs:label>
    <rdfs:comment>Properties of the instrument related to the wavelengths used for the observation.</rdfs:comment>
    <rdfs:subClassOf rdf:resource="https://schema.org/QuantitativeValue"/>
    <dcterms:source rdf:resource="http://docs.opengeospatial.org/is/17-003r2/17-003r2.html"/>
  </rdfs:Class>
   
   <!-- discreteWavelength ->  value -->
   <!--
   <rdf:Property rdf:about="https://schema.org/discreteWavelength">
    <schema:rangeIncludes rdf:resource="https://schema.org/Number"/>
    <schema:domainIncludes rdf:resource="https://schema.org/WavelengthInformation"/>
    <rdfs:label>discreteWavelengths</rdfs:label>
    <rdfs:comment>Discrete wavelength observed in the product.  Unit of measure is SI base unit (m) without prefix.</rdfs:comment>
    <dcterms:source rdf:resource="http://docs.opengeospatial.org/is/17-003r2/17-003r2.html"/>
  </rdf:Property>
   -->
  
  <!-- startWavelength -> minValue  -->
  <!-- endWavelength -> maxValue  -->
  
  <!--
   <rdf:Property rdf:about="https://schema.org/startWavelength">
    <schema:domainIncludes rdf:resource="https://schema.org/WavelengthInformation"/>
    <rdfs:comment>Start of the observed wavelength range.  Unit of measure is SI base unit (m) without prefix.</rdfs:comment>
    <dcterms:source rdf:resource="http://docs.opengeospatial.org/is/17-003r2/17-003r2.html"/>
    <rdfs:label>startWavelength</rdfs:label>
    <schema:rangeIncludes rdf:resource="https://schema.org/Number"/>
  </rdf:Property>
   
  <rdf:Property rdf:about="https://schema.org/endWavelength">
    <rdfs:comment>End of the observed wavelength range.  Unit of measure is SI base unit (m) without prefix.</rdfs:comment>
    <rdfs:label>endWavelength</rdfs:label>
    <schema:rangeIncludes rdf:resource="https://schema.org/Number"/>
    <dcterms:source rdf:resource="http://docs.opengeospatial.org/is/17-003r2/17-003r2.html"/>
    <schema:domainIncludes rdf:resource="https://schema.org/WavelengthInformation"/>
  </rdf:Property>
   -->
  
  <rdf:Property rdf:about="https://schema.org/spectralRange">
    <dcterms:source rdf:resource="http://docs.opengeospatial.org/is/17-003r2/17-003r2.html"/>
    <schema:domainIncludes rdf:resource="https://schema.org/WavelengthInformation"/>
    <rdfs:comment>The observed Spectral Range.</rdfs:comment>
    <rdfs:label>spectralRange</rdfs:label>
    <schema:rangeIncludes rdf:resource="https://schema.org/SpectralRangeType"/>
    <schema:rangeIncludes rdf:resource="https://schema.org/Text"/>
  </rdf:Property>
    
   <rdf:Property rdf:about="https://schema.org/wavelengthResolution">
    <rdfs:comment>Spacing between consecutive wavelengths.   Unit of measure is SI base unit (m) without prefix.</rdfs:comment>
    <dcterms:source rdf:resource="http://docs.opengeospatial.org/is/17-003r2/17-003r2.html"/>
    <schema:rangeIncludes rdf:resource="https://schema.org/Number"/>
    <rdfs:label>wavelengthResolution</rdfs:label>
    <schema:domainIncludes rdf:resource="https://schema.org/WavelengthInformation"/>
  </rdf:Property>
 
  <rdfs:Class rdf:about="https://schema.org/SpectralRangeType">
    <rdfs:comment>Enumeration of spectralRangeType constants.</rdfs:comment>
    <rdfs:label>SpectralRangeType</rdfs:label>
    <dcterms:source rdf:resource="http://docs.opengeospatial.org/is/17-003r2/17-003r2.html"/>
    <rdfs:subClassOf rdf:resource="https://schema.org/Enumeration"/>
  </rdfs:Class>
  
   <schema:SpectralRangeType rdf:about="https://schema.org/INFRARED">
    <rdfs:comment>SpectralRange type constant.</rdfs:comment>
    <rdfs:label>INFRARED</rdfs:label>
  </schema:SpectralRangeType>
  
  
  <schema:SpectralRangeType rdf:about="https://schema.org/SWIR">
    <rdfs:comment>SpectralRange type constant for Short Wavelength Infrared (SWIR).</rdfs:comment>
    <rdfs:label>SWIR</rdfs:label>
  </schema:SpectralRangeType>
  
   <schema:SpectralRangeType rdf:about="https://schema.org/VISIBLE">
    <rdfs:label>VISIBLE</rdfs:label>
    <rdfs:comment>SpectralRange type constant.</rdfs:comment>
  </schema:SpectralRangeType>
  
   <schema:SpectralRangeType rdf:about="https://schema.org/LWIR">
    <rdfs:label>LWIR</rdfs:label>
    <rdfs:comment>SpectralRange type constant for Long Wavelength Infrared (LWIR).</rdfs:comment>
  </schema:SpectralRangeType>
  
  <schema:SpectralRangeType rdf:about="https://schema.org/NIR">
    <rdfs:comment>SpectralRange type constant for Near Infrared (NIR).</rdfs:comment>
    <rdfs:label>NIR</rdfs:label>
  </schema:SpectralRangeType>
  
  <schema:SpectralRangeType rdf:about="https://schema.org/FIR">
    <rdfs:label>FIR</rdfs:label>
    <rdfs:comment>SpectralRange type constant for Far Infrared (FIR).</rdfs:comment>
  </schema:SpectralRangeType>
  
  <schema:SpectralRangeType rdf:about="https://schema.org/UV">
    <rdfs:label>UV</rdfs:label>
    <rdfs:comment>SpectralRange type constant for Ultraviolet (UV).</rdfs:comment>
  </schema:SpectralRangeType>
  
  <schema:SpectralRangeType rdf:about="https://schema.org/MWIR">
    <rdfs:label>MWIR</rdfs:label>
    <rdfs:comment>SpectralRange type constant for Mid Wavelength Infrared (MWIR).</rdfs:comment>
  </schema:SpectralRangeType>
  
  <schema:SpectralRangeType rdf:about="https://schema.org/MICROWAVE">
    <rdfs:comment>SpectralRange type constant.</rdfs:comment>
    <rdfs:label>MICROWAVE</rdfs:label>
  </schema:SpectralRangeType>
    
  <schema:SpectralRangeType rdf:about="https://schema.org/SR_OTHER">
    <rdfs:comment>SpectralRange type constant.</rdfs:comment>
    <rdfs:label>OTHER</rdfs:label>
  </schema:SpectralRangeType>
  
  
   <!-- §7.6.4   AcquisitionParameters  -->
   
  <rdfs:Class rdf:about="https://schema.org/AcquisitionParameters">
    <!-- <rdfs:subClassOf rdf:resource="https://schema.org/VerticalSpatialDomain"/>  -->
    <rdfs:comment>Contains the properties related to the acquisition of the data.</rdfs:comment>
    <rdfs:label>AcquisitionParameters</rdfs:label>
    <rdfs:subClassOf rdf:resource="https://schema.org/OrbitParameters"/>
  </rdfs:Class>
  
   <rdf:Property rdf:about="https://schema.org/location">
    <!-- <dcterms:source rdf:resource="http://docs.opengeospatial.org/is/17-003r2/17-003r2.html"/>  -->
    <schema:domainIncludes rdf:resource="https://schema.org/AcquisitionParameters"/>
  </rdf:Property>
  
  <rdf:Property rdf:about="https://schema.org/acquisitionType">
    <dcterms:source rdf:resource="http://docs.opengeospatial.org/is/17-003r2/17-003r2.html"/>
    <rdfs:label>acquisitionType</rdfs:label>
    <schema:rangeIncludes rdf:resource="https://schema.org/AcquisitionType"/>
    <rdfs:comment>AcquisitionType can be one of: 
 - NOMINAL
 - CALIBRATION
 - OTHER.</rdfs:comment>
    <schema:domainIncludes rdf:resource="https://schema.org/AcquisitionParameters"/>
  </rdf:Property>
  
  
  <rdfs:Class rdf:about="https://schema.org/AcquisitionType">
    <rdfs:label>AcquisitionType</rdfs:label>
    <rdfs:comment>Enumeration of acquisitionType constants.</rdfs:comment>
    <rdfs:subClassOf rdf:resource="https://schema.org/Enumeration"/>
    <dcterms:source rdf:resource="http://docs.opengeospatial.org/is/17-003r2/17-003r2.html"/>
  </rdfs:Class>
  
  <schema:AcquisitionType rdf:about="https://schema.org/NOMINAL">
    <rdfs:label>NOMINAL</rdfs:label>
    <rdfs:comment>Acquisition type constant.</rdfs:comment>
  </schema:AcquisitionType>
  
  <schema:AcquisitionType rdf:about="https://schema.org/CALIBRATION">
    <rdfs:label>CALIBRATION</rdfs:label>
    <rdfs:comment>Acquisition type constant.</rdfs:comment>
  </schema:AcquisitionType>
  
   <schema:AcquisitionType rdf:about="https://schema.org/ACQ_OTHER">
      <rdfs:comment>Acquisition type constant.</rdfs:comment>
      <rdfs:label>OTHER</rdfs:label>
  </schema:AcquisitionType>
  
  
  
   
  <rdf:Property rdf:about="https://schema.org/acquisitionSubType">
    <rdfs:comment>The broad value defined by the acquisitionType is too restrictive, so mission specific type definition should refer to mission/ground segment dedicated codeSpace.</rdfs:comment>
    <schema:rangeIncludes rdf:resource="https://schema.org/Text"/>
    <schema:domainIncludes rdf:resource="https://schema.org/AcquisitionParameters"/>
    <rdfs:label>acquisitionSubType</rdfs:label>
    <dcterms:source rdf:resource="http://docs.opengeospatial.org/is/17-003r2/17-003r2.html"/>
  </rdf:Property>
  
  
  <rdf:Property rdf:about="https://schema.org/startTimeFromAscendingNode">
    <rdfs:label>startTimeFromAscendingNode</rdfs:label>
    <schema:rangeIncludes rdf:resource="https://schema.org/Integer"/>
    <schema:domainIncludes rdf:resource="https://schema.org/AcquisitionParameters"/>
    <rdfs:comment>Start time of acquisition in milliseconds from ascending node date.</rdfs:comment>
    <dcterms:source rdf:resource="http://docs.opengeospatial.org/is/17-003r2/17-003r2.html"/>
  </rdf:Property>
  
  
  <rdf:Property rdf:about="https://schema.org/completionTimeFromAscendingNode">
    <rdfs:label>completionTimeFromAscendingNode</rdfs:label>
    <schema:domainIncludes rdf:resource="https://schema.org/AcquisitionParameters"/>
    <rdfs:comment>Stop time of acquisition in milliseconds from ascending node date.</rdfs:comment>
    <dcterms:source rdf:resource="http://docs.opengeospatial.org/is/17-003r2/17-003r2.html"/>
    <schema:rangeIncludes rdf:resource="https://schema.org/Integer"/>
  </rdf:Property>
  
  
    
  <rdf:Property rdf:about="https://schema.org/relativeOrbitNumber">
    <rdfs:comment>Orbit number since start of cycle.</rdfs:comment>
    <rdfs:label>relativeOrbitNumber</rdfs:label>
    <schema:rangeIncludes rdf:resource="https://schema.org/Integer"/>
    <schema:domainIncludes rdf:resource="https://schema.org/AcquisitionParameters"/>
    <dcterms:source rdf:resource="http://docs.opengeospatial.org/is/17-003r2/17-003r2.html"/>
  </rdf:Property>
  
    
  <rdf:Property rdf:about="https://schema.org/wrsLongitudeGrid">
    <schema:domainIncludes rdf:resource="https://schema.org/AcquisitionParameters"/>
    <schema:rangeIncludes rdf:resource="https://schema.org/Text"/>
    <dcterms:source rdf:resource="http://docs.opengeospatial.org/is/17-003r2/17-003r2.html"/>
    <rdfs:label>wrsLongitudeGrid</rdfs:label>
    <rdfs:comment>Neutral wrsLongitudeGrid equivalent to track in track/frame, K in K/J, etc.</rdfs:comment>
  </rdf:Property>
  
   <rdf:Property rdf:about="https://schema.org/wrsLatitudeGrid">
    <schema:domainIncludes rdf:resource="https://schema.org/AcquisitionParameters"/>
    <dcterms:source rdf:resource="http://docs.opengeospatial.org/is/17-003r2/17-003r2.html"/>
    <rdfs:comment>Neutral wrsLatitudeGrid equivalent to frame in track/frame,  J in K/J, etc.</rdfs:comment>
    <rdfs:label>wrsLatitudeGrid</rdfs:label>
    <schema:rangeIncludes rdf:resource="https://schema.org/Text"/>
  </rdf:Property>
  
  <rdf:Property rdf:about="https://schema.org/tileId">
    <schema:rangeIncludes rdf:resource="https://schema.org/Text"/>
    <rdfs:comment>While track/frame can be used to represent the first part of an MGRS coordinate (i.g. grid zone), the tileId identifies e.g. the second part of an MGRS coordinate (square identification), e.g. in case of Sentinel.
Used when the world reference system coordinates can not be expressed in X/Y (Track/Frame) terms, such has for UTM tiles. (used for Sentinel-2 L1C granules).</rdfs:comment>
    <dcterms:source rdf:resource="http://docs.opengeospatial.org/is/17-003r2/17-003r2.html"/>
    <schema:domainIncludes rdf:resource="https://schema.org/AcquisitionParameters"/>
    <rdfs:label>tileId</rdfs:label>
  </rdf:Property>
  
  
  <rdf:Property rdf:about="https://schema.org/groundTrackUncertainty">
    <schema:domainIncludes rdf:resource="https://schema.org/AcquisitionParameters"/>
    <dcterms:source rdf:resource="http://docs.opengeospatial.org/is/17-003r2/17-003r2.html"/>
    <rdfs:label>groundTrackUncertainty</rdfs:label>
    <rdfs:comment>Measure of the uncertainty of the ground track. Sometimes known as deadband e.g. 1000m (1Km) deadband.  Unit of measure is SI base unit (m) without prefix.</rdfs:comment>
    <schema:rangeIncludes rdf:resource="https://schema.org/Number"/>
  </rdf:Property>
  
    
  
  <rdf:Property rdf:about="https://schema.org/cycleNumber">
    <schema:domainIncludes rdf:resource="https://schema.org/AcquisitionParameters"/>
    <rdfs:label>cycleNumber</rdfs:label>
    <dcterms:source rdf:resource="http://docs.opengeospatial.org/is/17-003r2/17-003r2.html"/>
    <rdfs:comment>Number of Cycles.</rdfs:comment>
    <schema:rangeIncludes rdf:resource="https://schema.org/Integer"/>
  </rdf:Property>
  
    
  <rdf:Property rdf:about="https://schema.org/antennaLookDirection">
    <dcterms:source rdf:resource="http://docs.opengeospatial.org/is/17-003r2/17-003r2.html"/>
    <rdfs:comment>Look direction of antenna taken from codelist
Values:
- LEFT
- RIGHT.</rdfs:comment>
    <rdfs:label>antennaLookDirection</rdfs:label>
    <schema:rangeIncludes rdf:resource="https://schema.org/AntennaLookDirectionType"/>
    <schema:domainIncludes rdf:resource="https://schema.org/AcquisitionParameters"/>
  </rdf:Property>
  
   <rdfs:Class rdf:about="https://schema.org/AntennaLookDirectionType">
    <dcterms:source rdf:resource="http://docs.opengeospatial.org/is/17-003r2/17-003r2.html"/>
    <rdfs:subClassOf rdf:resource="https://schema.org/Enumeration"/>
    <rdfs:comment>Enumeration of antennaLookDirectionType constants.</rdfs:comment>
    <rdfs:label>AntennaLookDirectionType</rdfs:label>
  </rdfs:Class>
  
  <schema:AntennaLookDirectionType rdf:about="https://schema.org/LEFT">
    <rdfs:comment>Antenna look direction constant.</rdfs:comment>
    <rdfs:label>LEFT</rdfs:label>
  </schema:AntennaLookDirectionType>
  
     <schema:AntennaLookDirectionType rdf:about="https://schema.org/RIGHT">
    <rdfs:label>RIGHT</rdfs:label>
    <rdfs:comment>Antenna look direction constant.</rdfs:comment>
  </schema:AntennaLookDirectionType>
  
  
   <rdf:Property rdf:about="https://schema.org/acquisitionStation">
    <schema:domainIncludes rdf:resource="https://schema.org/AcquisitionParameters"/>
    <rdfs:label>acquisitionStation</rdfs:label>
    <dcterms:source rdf:resource="http://docs.opengeospatial.org/is/17-003r2/17-003r2.html"/>
    <rdfs:comment>Acquisition / receiving station code. Possible values are mission specific and should be retrieved using codespace.</rdfs:comment>
    <schema:rangeIncludes rdf:resource="https://schema.org/Text"/>
  </rdf:Property>
  
  
   <rdf:Property rdf:about="https://schema.org/acquisitionAngles">
    <schema:domainIncludes rdf:resource="https://schema.org/AcquisitionParameters"/>
    <dcterms:source rdf:resource="http://docs.opengeospatial.org/is/17-003r2/17-003r2.html"/>
    <rdfs:comment>Acquisition angles.</rdfs:comment>
    <schema:rangeIncludes rdf:resource="https://schema.org/AcquisitionAngles"/>
    <rdfs:label>acquisitionAngles</rdfs:label>
  </rdf:Property>
  
  
   <rdf:Property rdf:about="https://schema.org/operationalMode">
    <schema:rangeIncludes rdf:resource="https://schema.org/Text"/>
    <schema:domainIncludes rdf:resource="https://schema.org/AcquisitionParameters"/>
    <dcterms:source rdf:resource="http://docs.opengeospatial.org/is/17-003r2/17-003r2.html"/>
    <rdfs:label>operationalMode</rdfs:label>
    <rdfs:comment>Sensor mode. Possible values are mission specific.</rdfs:comment>
  </rdf:Property>
  
  
  <rdf:Property rdf:about="https://schema.org/swathIdentifier">
    <rdfs:label>swathIdentifier</rdfs:label>
    <schema:domainIncludes rdf:resource="https://schema.org/AcquisitionParameters"/>
    <schema:rangeIncludes rdf:resource="https://schema.org/Text"/>
    <rdfs:comment>Swath identifier (e.g. Envisat ASAR has 7 distinct swaths (I1,I2,I3...I7) that correspond to precise incidence angles for the sensor).</rdfs:comment>
    <dcterms:source rdf:resource="http://docs.opengeospatial.org/is/17-003r2/17-003r2.html"/>
  </rdf:Property>
  
  
  <rdf:Property rdf:about="https://schema.org/polarisationMode">
    <schema:rangeIncludes rdf:resource="https://schema.org/PolarisationModeType"/>
    <schema:domainIncludes rdf:resource="https://schema.org/AcquisitionParameters"/>
    <dcterms:source rdf:resource="http://docs.opengeospatial.org/is/17-003r2/17-003r2.html"/>
    <rdfs:label>polarisationMode</rdfs:label>
    <rdfs:comment>Polarisation mode taken from codelist:
S (for single),
D (for dual),
T (for twin),
Q (for quad),
UNDEFINED.</rdfs:comment>
  </rdf:Property>
  
 <rdfs:Class rdf:about="https://schema.org/PolarisationModeType">
    <rdfs:subClassOf rdf:resource="https://schema.org/Enumeration"/>
    <rdfs:comment>Enumeration of polarisationMode constants.</rdfs:comment>
    <rdfs:label>PolarisationModeType</rdfs:label>
    <dcterms:source rdf:resource="http://docs.opengeospatial.org/is/17-003r2/17-003r2.html"/>
  </rdfs:Class>
   
  <schema:PolarisationModeType rdf:about="https://schema.org/Q">
    <rdfs:label>Q</rdfs:label>
    <rdfs:comment>Polarisation mode constant (Quad).</rdfs:comment>
  </schema:PolarisationModeType>
  
  <schema:PolarisationModeType rdf:about="https://schema.org/S">
    <rdfs:label>S</rdfs:label>
    <rdfs:comment>Polarisation mode constant (Single).</rdfs:comment>
  </schema:PolarisationModeType>
  
  <schema:PolarisationModeType rdf:about="https://schema.org/D">
    <rdfs:label>D</rdfs:label>
    <rdfs:comment>Polarisation mode constant (Dual).</rdfs:comment>
  </schema:PolarisationModeType>
  
  <schema:PolarisationModeType rdf:about="https://schema.org/T">
    <rdfs:label>T</rdfs:label>
    <rdfs:comment>Polarisation mode constant (Twin).</rdfs:comment>
  </schema:PolarisationModeType>
    
 <schema:PolarisationModeType rdf:about="https://schema.org/PM_UNDEFINED">
    <rdfs:comment>Polarisation mode constant.</rdfs:comment>
    <rdfs:label>UNDEFINED</rdfs:label>
  </schema:PolarisationModeType>  
  
 
    
  <rdf:Property rdf:about="https://schema.org/polarisationChannels">
    <schema:domainIncludes rdf:resource="https://schema.org/AcquisitionParameters"/>
    <rdfs:comment>Polarisation channel transmit/receive configuration.</rdfs:comment>
    <dcterms:source rdf:resource="http://docs.opengeospatial.org/is/17-003r2/17-003r2.html"/>
    <schema:rangeIncludes rdf:resource="https://schema.org/PolarisationChannelsType"/>
    <rdfs:label>polarisationChannels</rdfs:label>
  </rdf:Property>
    
  <rdfs:Class rdf:about="https://schema.org/PolarisationChannelsType">
    <rdfs:label>PolarisationChannelsType</rdfs:label>
    <dcterms:source rdf:resource="http://docs.opengeospatial.org/is/17-003r2/17-003r2.html"/>
    <rdfs:subClassOf rdf:resource="https://schema.org/Enumeration"/>
    <rdfs:comment>Enumeration of polarisationChannels constants.</rdfs:comment>
  </rdfs:Class>
  
  <schema:PolarisationChannelsType rdf:about="https://schema.org/HH_VV">
    <rdfs:label>HH_VV</rdfs:label>
    <rdfs:comment>Polarisation channel constant.</rdfs:comment>
  </schema:PolarisationChannelsType>
  
  <schema:PolarisationChannelsType rdf:about="https://schema.org/HH_VH">
    <rdfs:comment>Polarisation channel constant.</rdfs:comment>
    <rdfs:label>HH_VH</rdfs:label>
  </schema:PolarisationChannelsType>
  
  <schema:PolarisationChannelsType rdf:about="https://schema.org/VH_VV">
    <rdfs:label>VH_VV</rdfs:label>
    <rdfs:comment>Polarisation channel constant.</rdfs:comment>
  </schema:PolarisationChannelsType>
  
  <schema:PolarisationChannelsType rdf:about="https://schema.org/HH">
    <rdfs:comment>Polarisation channel constant.</rdfs:comment>
    <rdfs:label>HH</rdfs:label>
  </schema:PolarisationChannelsType>
  
  <schema:PolarisationChannelsType rdf:about="https://schema.org/VH">
    <rdfs:comment>Polarisation channel constant.</rdfs:comment>
    <rdfs:label>VH</rdfs:label>
  </schema:PolarisationChannelsType>
  
  <schema:PolarisationChannelsType rdf:about="https://schema.org/VV_HV">
    <rdfs:comment>Polarisation channel constant.</rdfs:comment>
    <rdfs:label>VV_HV</rdfs:label>
  </schema:PolarisationChannelsType>
   
  <schema:PolarisationChannelsType rdf:about="https://schema.org/HH_HV">
    <rdfs:label>HH_HV</rdfs:label>
    <rdfs:comment>Polarisation channel constant.</rdfs:comment>
  </schema:PolarisationChannelsType>
  
  <schema:PolarisationChannelsType rdf:about="https://schema.org/VV_VH">
    <rdfs:label>VV_VH</rdfs:label>
    <rdfs:comment>Polarisation channel constant.</rdfs:comment>
  </schema:PolarisationChannelsType>
  
  <schema:PolarisationChannelsType rdf:about="https://schema.org/VH_HV">
    <rdfs:comment>Polarisation channel constant.</rdfs:comment>
    <rdfs:label>VH_HV</rdfs:label>
  </schema:PolarisationChannelsType>
  
  <schema:PolarisationChannelsType rdf:about="https://schema.org/HH_HV_VH_VV">
    <rdfs:comment>Polarisation channel constant.</rdfs:comment>
    <rdfs:label>HH_HV_VH_VV</rdfs:label>
  </schema:PolarisationChannelsType>
  
    <schema:PolarisationChannelsType rdf:about="https://schema.org/HV_VH">
    <rdfs:label>HV_VH</rdfs:label>
    <rdfs:comment>Polarisation channel constant.</rdfs:comment>
  </schema:PolarisationChannelsType>
  
  <schema:PolarisationChannelsType rdf:about="https://schema.org/HV">
    <rdfs:label>HV</rdfs:label>
    <rdfs:comment>Polarisation channel constant.</rdfs:comment>
  </schema:PolarisationChannelsType>
  
  <schema:PolarisationChannelsType rdf:about="https://schema.org/VV">
    <rdfs:comment>Polarisation channel constant.</rdfs:comment>
    <rdfs:label>VV</rdfs:label>
  </schema:PolarisationChannelsType>
       
  <schema:PolarisationChannelsType rdf:about="https://schema.org/PC_UNDEFINED">
    <rdfs:label>UNDEFINED</rdfs:label>
    <rdfs:comment>Polarisation channel constant.</rdfs:comment>
  </schema:PolarisationChannelsType>
  
     
   <rdf:Property rdf:about="https://schema.org/resolution">
    <dcterms:source rdf:resource="http://docs.opengeospatial.org/is/17-003r2/17-003r2.html"/>
    <rdfs:comment>Sensor resolution.  Unit of measure is SI base unit (m) without prefix.</rdfs:comment>
    <rdfs:label>resolution</rdfs:label>
    <schema:domainIncludes rdf:resource="https://schema.org/AcquisitionParameters"/>
    <schema:rangeIncludes rdf:resource="https://schema.org/Number"/>
  </rdf:Property>
    
  
   <rdf:Property rdf:about="https://schema.org/verticalResolution">
    <dcterms:source rdf:resource="http://docs.opengeospatial.org/is/17-003r2/17-003r2.html"/>
    <rdfs:comment>lmb: Vertical spacing of data (if regular)
atm: Full width at half maximum of the rows of the vertical averaging kernel matrix
Unit of measure is SI base unit (m) without prefix.</rdfs:comment>
    <rdfs:label>verticalResolution</rdfs:label>
    <schema:rangeIncludes rdf:resource="https://schema.org/Number"/>
    <schema:domainIncludes rdf:resource="https://schema.org/AcquisitionParameters"/>
  </rdf:Property>
  
  
  <rdf:Property rdf:about="https://schema.org/wavelengths">
    <rdfs:label>wavelengths</rdfs:label>
    <dcterms:source rdf:resource="http://docs.opengeospatial.org/is/17-003r2/17-003r2.html"/>
    <rdfs:comment>List of discrete wavelengths observed in the product.</rdfs:comment>
    <schema:rangeIncludes rdf:resource="https://schema.org/WavelengthInformation"/>
    <schema:domainIncludes rdf:resource="https://schema.org/AcquisitionParameters"/>
  </rdf:Property>
     
   
  <rdf:Property rdf:about="https://schema.org/measurementType">
    <schema:rangeIncludes rdf:resource="https://schema.org/MeasurementType"/>
    <schema:domainIncludes rdf:resource="https://schema.org/AcquisitionParameters"/>
    <dcterms:source rdf:resource="http://docs.opengeospatial.org/is/17-003r2/17-003r2.html"/>
    <rdfs:label>measurementType</rdfs:label>
    <rdfs:comment>Measurement type taken from codelist:
Values:
- ABSORPTION
- EMISSION.</rdfs:comment>
  </rdf:Property>
  
    <rdfs:Class rdf:about="https://schema.org/MeasurementType">
    <rdfs:label>MeasurementType</rdfs:label>
    <rdfs:subClassOf rdf:resource="https://schema.org/Enumeration"/>
    <dcterms:source rdf:resource="http://docs.opengeospatial.org/is/17-003r2/17-003r2.html"/>
    <rdfs:comment>Enumeration of measurementType constants.</rdfs:comment>
  </rdfs:Class>
  
  <schema:MeasurementType rdf:about="https://schema.org/EMISSION">
    <rdfs:label>EMISSION</rdfs:label>
    <rdfs:comment>Measurement type constant (Emission).</rdfs:comment>
  </schema:MeasurementType>
  
  <schema:MeasurementType rdf:about="https://schema.org/ABSORPTION">
    <rdfs:label>ABSORPTION</rdfs:label>
    <rdfs:comment>Measurement type constant (Absorption).</rdfs:comment>
  </schema:MeasurementType>
  
       
       
  
   <rdf:Property rdf:about="https://schema.org/dopplerFrequency">
    <rdfs:label>dopplerFrequency</rdfs:label>
    <dcterms:source rdf:resource="http://docs.opengeospatial.org/is/17-003r2/17-003r2.html"/>
    <rdfs:comment>Doppler Frequency of acquisition.   Unit of measure is SI base unit (m) without prefix.</rdfs:comment>
    <schema:rangeIncludes rdf:resource="https://schema.org/Number"/>
    <schema:domainIncludes rdf:resource="https://schema.org/AcquisitionParameters"/>
  </rdf:Property>
  
    
  <rdf:Property rdf:about="https://schema.org/samplingRate">
    <schema:rangeIncludes rdf:resource="https://schema.org/Number"/>
    <dcterms:source rdf:resource="http://docs.opengeospatial.org/is/17-003r2/17-003r2.html"/>
    <rdfs:comment>Rate at which samples are provided in product. Some products may contain more than one sampling rate, e.g. 1kHz and 20kHz. Cardinality is therefore zero to many.  Unit of measure (Hz) is SI derived unit without prefix.</rdfs:comment>
    <rdfs:label>samplingRates</rdfs:label>
    <schema:domainIncludes rdf:resource="https://schema.org/AcquisitionParameters"/>
  </rdf:Property>
  
  

  
   <!-- §7.6.5   AcquisitionAngles  -->
  
   <rdfs:Class rdf:about="https://schema.org/AcquisitionAngles">
    <rdfs:label>AcquisitionAngles</rdfs:label>
    <dcterms:source rdf:resource="http://docs.opengeospatial.org/is/17-003r2/17-003r2.html"/>
    <rdfs:comment>Contains the properties related to the acquisition angles.</rdfs:comment>
    <rdfs:subClassOf rdf:resource="https://schema.org/StructuredValue"/>
  </rdfs:Class>
  
  
  
  <rdf:Property rdf:about="https://schema.org/illuminationAzimuthAngle">
    <schema:domainIncludes rdf:resource="https://schema.org/AcquisitionAngles"/>
    <dcterms:source rdf:resource="http://docs.opengeospatial.org/is/17-003r2/17-003r2.html"/>
    <rdfs:label>illuminationAzimuthAngle</rdfs:label>
    <schema:rangeIncludes rdf:resource="https://schema.org/Number"/>
    <rdfs:comment>Mean illumination/solar azimuth angle given in degrees (i.e. uom='deg').</rdfs:comment>
  </rdf:Property>
 
 <rdf:Property rdf:about="https://schema.org/illuminationZenithAngle">
    <schema:domainIncludes rdf:resource="https://schema.org/AcquisitionAngles"/>
    <rdfs:label>illuminationZenithAngle</rdfs:label>
    <schema:rangeIncludes rdf:resource="https://schema.org/Number"/>
    <rdfs:comment>Mean illumination/solar zenith angle in degrees (i.e. uom='deg').</rdfs:comment>
    <dcterms:source rdf:resource="http://docs.opengeospatial.org/is/17-003r2/17-003r2.html"/>
  </rdf:Property>
  
  <rdf:Property rdf:about="https://schema.org/illuminationElevationAngle">
    <schema:rangeIncludes rdf:resource="https://schema.org/Number"/>
    <dcterms:source rdf:resource="http://docs.opengeospatial.org/is/17-003r2/17-003r2.html"/>
    <rdfs:comment>Mean illumination/solar elevation angle in degrees (i.e. uom='deg').</rdfs:comment>
    <schema:domainIncludes rdf:resource="https://schema.org/AcquisitionAngles"/>
    <rdfs:label>illuminationElevationAngle</rdfs:label>
  </rdf:Property>
    
  
  
  <rdf:Property rdf:about="https://schema.org/incidenceAngle">
    <schema:rangeIncludes rdf:resource="https://schema.org/QuantitativeValue"/>
    <dcterms:source rdf:resource="http://docs.opengeospatial.org/is/17-003r2/17-003r2.html"/>
    <rdfs:label>incidenceAngle</rdfs:label>
    <schema:domainIncludes rdf:resource="https://schema.org/AcquisitionAngles"/>
    <rdfs:comment>Acquisition global incidence angle in degrees (i.e. uom='deg'), its minimum value and its maximum value.</rdfs:comment>
  </rdf:Property>
  
    
  <rdf:Property rdf:about="https://schema.org/incidenceAngleVariation">
    <dcterms:source rdf:resource="http://docs.opengeospatial.org/is/17-003r2/17-003r2.html"/>
    <schema:rangeIncludes rdf:resource="https://schema.org/Number"/>
    <schema:domainIncludes rdf:resource="https://schema.org/AcquisitionAngles"/>
    <rdfs:label>incidenceAngleVariation</rdfs:label>
    <rdfs:comment>Incidence angle variation in degrees (i.e. uom='deg').</rdfs:comment>
  </rdf:Property>
  
  
  <rdf:Property rdf:about="https://schema.org/acrossTrackIncidenceAngle">
    <rdfs:label>acrossTrackIncidenceAngle</rdfs:label>
    <dcterms:source rdf:resource="http://docs.opengeospatial.org/is/17-003r2/17-003r2.html"/>
    <rdfs:comment>Acquisition across track incidence angle in degrees (i.e. uom='deg').</rdfs:comment>
    <schema:domainIncludes rdf:resource="https://schema.org/AcquisitionAngles"/>
    <schema:rangeIncludes rdf:resource="https://schema.org/Number"/>
  </rdf:Property>

  
  <rdf:Property rdf:about="https://schema.org/alongTrackIncidenceAngle">
    <schema:domainIncludes rdf:resource="https://schema.org/AcquisitionAngles"/>
    <schema:rangeIncludes rdf:resource="https://schema.org/Number"/>
    <dcterms:source rdf:resource="http://docs.opengeospatial.org/is/17-003r2/17-003r2.html"/>
    <rdfs:label>alongTrackIncidenceAngle</rdfs:label>
    <rdfs:comment>Acquisition along track incidence angle in degrees (i.e. uom='deg').</rdfs:comment>
  </rdf:Property>
  
    
  
   <rdf:Property rdf:about="https://schema.org/instrumentAzimuthAngle">
    <dcterms:source rdf:resource="http://docs.opengeospatial.org/is/17-003r2/17-003r2.html"/>
    <rdfs:comment>Mean instrument azimuth angle in degrees (i.e. uom='deg').</rdfs:comment>
    <rdfs:label>instrumentAzimuthAngle</rdfs:label>
    <schema:domainIncludes rdf:resource="https://schema.org/AcquisitionAngles"/>
    <schema:rangeIncludes rdf:resource="https://schema.org/Number"/>
  </rdf:Property>
    
  
  <rdf:Property rdf:about="https://schema.org/instrumentZenithAngle">
    <rdfs:label>instrumentZenithAngle</rdfs:label>
    <schema:domainIncludes rdf:resource="https://schema.org/AcquisitionAngles"/>
    <schema:rangeIncludes rdf:resource="https://schema.org/Number"/>
    <rdfs:comment>Mean instrument zenith angle in degrees (i.e. uom='deg').</rdfs:comment>
    <dcterms:source rdf:resource="http://docs.opengeospatial.org/is/17-003r2/17-003r2.html"/>
  </rdf:Property>
  
  
  <rdf:Property rdf:about="https://schema.org/instrumentElevationAngle">
    <rdfs:comment>Mean instrument elevation angle in degrees (i.e. uom='deg').</rdfs:comment>
    <dcterms:source rdf:resource="http://docs.opengeospatial.org/is/17-003r2/17-003r2.html"/>
    <schema:domainIncludes rdf:resource="https://schema.org/AcquisitionAngles"/>
    <rdfs:label>instrumentElevationAngle</rdfs:label>
    <schema:rangeIncludes rdf:resource="https://schema.org/Number"/>
  </rdf:Property>
  
  
  <rdf:Property rdf:about="https://schema.org/pitch">
    <dcterms:source rdf:resource="http://docs.opengeospatial.org/is/17-003r2/17-003r2.html"/>
    <rdfs:comment>Satellite pitch angle in degrees (i.e. uom='deg').</rdfs:comment>
    <schema:domainIncludes rdf:resource="https://schema.org/AcquisitionAngles"/>
    <rdfs:label>pitch</rdfs:label>
    <schema:rangeIncludes rdf:resource="https://schema.org/Number"/>
  </rdf:Property>
  
   <rdf:Property rdf:about="https://schema.org/roll">
    <schema:rangeIncludes rdf:resource="https://schema.org/Number"/>
    <rdfs:comment>Satellite roll angle in degrees (i.e. uom='deg').</rdfs:comment>
    <dcterms:source rdf:resource="http://docs.opengeospatial.org/is/17-003r2/17-003r2.html"/>
    <rdfs:label>roll</rdfs:label>
    <schema:domainIncludes rdf:resource="https://schema.org/AcquisitionAngles"/>
  </rdf:Property>
  
    
  <rdf:Property rdf:about="https://schema.org/yaw">
    <rdfs:comment>Satellite yaw angle in degrees (i.e. uom='deg').</rdfs:comment>
    <schema:domainIncludes rdf:resource="https://schema.org/AcquisitionAngles"/>
    <rdfs:label>yaw</rdfs:label>
    <schema:rangeIncludes rdf:resource="https://schema.org/Number"/>
    <dcterms:source rdf:resource="http://docs.opengeospatial.org/is/17-003r2/17-003r2.html"/>
  </rdf:Property>
  
  
  
    <!-- §7.7   ProductInformation  -->
    
    
  <rdfs:Class rdf:about="https://schema.org/ProductInformation">
    <rdfs:subClassOf rdf:resource="https://schema.org/CoverageDescription"/>
    <rdfs:subClassOf rdf:resource="https://schema.org/ProcessingInformation"/>
    <rdfs:subClassOf rdf:resource="https://schema.org/StructuredValue"/>
    <rdfs:label>ProductInformation</rdfs:label>
    <rdfs:comment>Product information of the Earth Observation product as defined in OGC 17-003r2.</rdfs:comment>
    <dcterms:source rdf:resource="http://docs.opengeospatial.org/is/17-003r2/17-003r2.html"/>
    <owl:equivalentClass rdf:resource="http://www.opengis.net/ont/eo-geojson/1.0/ProductInformation"/>
  </rdfs:Class>
  
  <rdf:Property rdf:about="https://schema.org/productType">
    <schema:rangeIncludes rdf:resource="https://schema.org/Text"/>
    <dcterms:source rdf:resource="http://docs.opengeospatial.org/is/17-003r2/17-003r2.html"/>
    <owl:equivalentProperty rdf:resource="http://www.opengis.net/ont/eo-geojson/1.0/productType"/>
    <rdfs:comment>Describes the product type in case that mixed types are available within a single collection, this is a ground segment specific definition.</rdfs:comment>
    <rdfs:label>productType</rdfs:label>
    <schema:domainIncludes rdf:resource="https://schema.org/ProductInformation"/>
  </rdf:Property>
  
  <rdf:Property rdf:about="https://schema.org/contentSize">
    <schema:domainIncludes rdf:resource="https://schema.org/ProductInformation"/>
    <!-- <owl:equivalentProperty rdf:resource="http://www.opengis.net/ont/eo-geojson/1.0/size"/> -->
  </rdf:Property>
  
   <rdf:Property rdf:about="https://schema.org/statusSubType">
    <rdfs:comment>Refines the status of a product when the “status” is set to “ARCHIVED”.  
Possible values:
- “ON-LINE”
- “OFF-LINE”.</rdfs:comment>
    <rdfs:label>statusSubType</rdfs:label>
    <dcterms:source rdf:resource="http://docs.opengeospatial.org/is/17-003r2/17-003r2.html"/>
    <schema:domainIncludes rdf:resource="https://schema.org/ProductInformation"/>
    <schema:rangeIncludes rdf:resource="https://schema.org/Text"/>
  </rdf:Property>
  
  
  
  <rdf:Property rdf:about="https://schema.org/statusDetail">
    <rdfs:label>statusDetail</rdfs:label>
    <rdfs:comment>This field refers to the status value. It should be used to motivate the reason of a failure, cancelation, rejection or degraded quality.</rdfs:comment>
    <schema:domainIncludes rdf:resource="https://schema.org/ProductInformation"/>
    <schema:rangeIncludes rdf:resource="https://schema.org/Text"/>
    <dcterms:source rdf:resource="http://docs.opengeospatial.org/is/17-003r2/17-003r2.html"/>
  </rdf:Property>
  
   <rdf:Property rdf:about="https://schema.org/availabilityTime">
    <rdfs:label>availabilityTime</rdfs:label>
    <schema:rangeIncludes rdf:resource="https://schema.org/DateTime"/>
    <rdfs:comment>The time when the result becomes available
 dateTime in ISO 8601 format (CCYY-MM-DDThh:mm[:ss[.cc]]Z).</rdfs:comment>
    <schema:domainIncludes rdf:resource="https://schema.org/ProductInformation"/>
    <dcterms:source rdf:resource="http://docs.opengeospatial.org/is/17-003r2/17-003r2.html"/>
  </rdf:Property>
  
   
  
  <rdf:Property rdf:about="https://schema.org/timeliness">
    <rdfs:comment>Timeliness of the product, such as "near real time", "rush". Possible values are mission specific and shall refer to mission/ground segment dedicated codeSpace.
Example of values could be "NRT", "NOMINAL", “NTC” or “STC”.</rdfs:comment>
    <dcterms:source rdf:resource="http://docs.opengeospatial.org/is/17-003r2/17-003r2.html"/>
    <schema:domainIncludes rdf:resource="https://schema.org/ProductInformation"/>
    <schema:rangeIncludes rdf:resource="https://schema.org/Text"/>
    <rdfs:label>timeliness</rdfs:label>
  </rdf:Property>
  
  
  <!-- productGroupId -->
  <rdf:Property rdf:about="https://schema.org/isPartOf">
      <schema:domainIncludes rdf:resource="https://schema.org/ProductInformation"/>
    <!-- <owl:equivalentProperty rdf:resource="http://www.opengis.net/ont/eo-geojson/1.0/productGroupId"/> -->
  </rdf:Property>
  
    
  <!-- productVersion -->
  <!-- TBD: associate to the Dataset instead ? -->
  <rdf:Property rdf:about="https://schema.org/version">
    <schema:domainIncludes rdf:resource="https://schema.org/ProductInformation"/>
    <!--  <owl:equivalentProperty rdf:resource="http://www.opengis.net/ont/eo-geojson/1.0/productVersion"/>  -->
  </rdf:Property>
  
  <!-- archivingCenter -->  
  <rdf:Property rdf:about="https://schema.org/holdingArchive">
    <schema:domainIncludes rdf:resource="https://schema.org/ProductInformation"/>
    <!-- <owl:equivalentProperty rdf:resource="http://www.opengis.net/ont/eo-geojson/1.0/archivingCenter"/> -->
  </rdf:Property>
  
    
  <rdf:Property rdf:about="https://schema.org/archivingDate">
    <rdfs:comment>Archiving date time.</rdfs:comment>
    <schema:domainIncludes rdf:resource="https://schema.org/ProductInformation"/>
    <dcterms:source rdf:resource="http://docs.opengeospatial.org/is/17-003r2/17-003r2.html"/>
    <schema:rangeIncludes rdf:resource="https://schema.org/DateTime"/>
    <rdfs:label>archivingDate</rdfs:label>
  </rdf:Property>
  
 
  <!-- referenceSystemIdentifier ->  additionalProperty --> 
   
    <rdf:Property rdf:about="https://schema.org/qualityInformation">
    <schema:domainIncludes rdf:resource="https://schema.org/ProductInformation"/>
    <schema:rangeIncludes rdf:resource="https://schema.org/QualityInformation"/>
    <dcterms:source rdf:resource="http://docs.opengeospatial.org/is/17-003r2/17-003r2.html"/>
    <rdfs:label>qualityInformation</rdfs:label>
    <rdfs:comment>Contains properties related to the quality of the product.</rdfs:comment>
  </rdf:Property>
  
 
 
   <!-- §7.7.1   QualityInformation  -->
  
  
  <rdfs:Class rdf:about="https://schema.org/QualityInformation">
    <dcterms:source rdf:resource="http://docs.opengeospatial.org/is/17-003r2/17-003r2.html"/>
    <rdfs:comment>Contains the properties related to the quality of the product.</rdfs:comment>
    <owl:equivalentClass rdf:resource="http://www.opengis.net/ont/eo-geojson/1.0/QualityInformation"/>
    <rdfs:label>QualityInformation</rdfs:label>
    <rdfs:subClassOf rdf:resource="https://schema.org/StructuredValue"/>
  </rdfs:Class>
  
   <rdf:Property rdf:about="https://schema.org/qualityStatus">
    <schema:domainIncludes rdf:resource="https://schema.org/QualityInformation"/>
    <rdfs:label>qualityStatus</rdfs:label>
    <schema:rangeIncludes rdf:resource="https://schema.org/Text"/>
    <rdfs:comment>Indicator that specifies whether the product quality is degraded or not.  This optional field shall be provided if the product has passed a quality check.
Values:
DEGRADED, NOMINAL.</rdfs:comment>
    <dcterms:source rdf:resource="http://docs.opengeospatial.org/is/17-003r2/17-003r2.html"/>
  </rdf:Property>
     
  
  <rdf:Property rdf:about="https://schema.org/qualityDegradation">
    <schema:domainIncludes rdf:resource="https://schema.org/QualityInformation"/>
    <dcterms:source rdf:resource="http://docs.opengeospatial.org/is/17-003r2/17-003r2.html"/>
    <rdfs:label>qualityDegradation</rdfs:label>
    <rdfs:comment>Quality degradation percentage (i.e. uom=’%’).</rdfs:comment>
    <schema:rangeIncludes rdf:resource="https://schema.org/Number"/>
  </rdf:Property>
 
       
  <rdf:Property rdf:about="https://schema.org/qualityDegradationQuotationMode">
    <rdfs:comment>Indicator to know how the quality degradation percentage has been calculated.
Values:
AUTOMATIC, MANUAL.</rdfs:comment>
    <schema:rangeIncludes rdf:resource="https://schema.org/Text"/>
    <schema:domainIncludes rdf:resource="https://schema.org/QualityInformation"/>
    <rdfs:label>qualityDegradationQuotationMode</rdfs:label>
    <dcterms:source rdf:resource="http://docs.opengeospatial.org/is/17-003r2/17-003r2.html"/>
  </rdf:Property>
     
  
  <rdf:Property rdf:about="https://schema.org/qualityDegradationTag">
    <schema:domainIncludes rdf:resource="https://schema.org/QualityInformation"/>
    <schema:rangeIncludes rdf:resource="https://schema.org/Text"/>
    <dcterms:source rdf:resource="http://docs.opengeospatial.org/is/17-003r2/17-003r2.html"/>
    <rdfs:label>qualityDegradationTag</rdfs:label>
    <rdfs:comment>Contains further textual information concerning the quality degradation.  It shall be provided if qualityStatus value is DEGRADED. Possible values are mission specific and should refer to mission/ground segment dedicated codeSpace.
Example of values could be "RADIOMETRY" or "GEOLOCATION".</rdfs:comment>
  </rdf:Property>
  
  
    <!-- §7.7.2   ProcessingInformation  -->
    
    
    
  <rdfs:Class rdf:about="https://schema.org/ProcessingInformation">
    <rdfs:subClassOf rdf:resource="https://schema.org/StructuredValue"/>
    <rdfs:comment>Contains the properties related to the processing of the data.</rdfs:comment>
    <rdfs:label>ProcessingInformation</rdfs:label>
    <dcterms:source rdf:resource="http://docs.opengeospatial.org/is/17-003r2/17-003r2.html"/>
    <owl:equivalentClass rdf:resource="http://www.opengis.net/ont/eo-geojson/1.0/ProcessingInformation"/>
  </rdfs:Class>
   
  <rdf:Property rdf:about="https://schema.org/compositeType">
    <schema:domainIncludes rdf:resource="https://schema.org/ProcessingInformation"/>
    <schema:rangeIncludes rdf:resource="https://schema.org/Duration"/>
    <dcterms:source rdf:resource="http://docs.opengeospatial.org/is/17-003r2/17-003r2.html"/>
    <rdfs:seeAlso rdf:resource="https://en.wikipedia.org/wiki/ISO_8601#Durations"/>
    <rdfs:comment>Type of composite product expressed as timeperiod that the composite product covers using ISO 8601 duration format P[n]Y[n]M[n]D encoding , e.g. P10D for a 10 day composite.</rdfs:comment>
    <rdfs:label>compositeType</rdfs:label>
  </rdf:Property>
  
  
  <!-- format ? -->
  
    
  <rdf:Property rdf:about="https://schema.org/processingMethod">
    <rdfs:label>processingMethod</rdfs:label>
    <rdfs:comment>Method used to compute datalayer. (e.g. Kalman filtering, ROSE).</rdfs:comment>
    <schema:domainIncludes rdf:resource="https://schema.org/ProcessingInformation"/>
    <dcterms:source rdf:resource="http://docs.opengeospatial.org/is/17-003r2/17-003r2.html"/>
    <schema:rangeIncludes rdf:resource="https://schema.org/Text"/>
  </rdf:Property>
  
  
  <rdf:Property rdf:about="https://schema.org/processingMethodVersion">
    <rdfs:label>processingMethodVersion</rdfs:label>
    <dcterms:source rdf:resource="http://docs.opengeospatial.org/is/17-003r2/17-003r2.html"/>
    <rdfs:comment>Method version (e.g. 1.0).</rdfs:comment>
    <schema:rangeIncludes rdf:resource="https://schema.org/Text"/>
    <schema:domainIncludes rdf:resource="https://schema.org/ProcessingInformation"/>
  </rdf:Property>
  
    
  <rdf:Property rdf:about="https://schema.org/processingCenter">
    <schema:domainIncludes rdf:resource="https://schema.org/ProcessingInformation"/>
    <schema:rangeIncludes rdf:resource="https://schema.org/Text"/>
    <rdfs:comment>Processing center code. Possible values are mission specific.</rdfs:comment>
    <rdfs:label>processingCenter</rdfs:label>
    <dcterms:source rdf:resource="http://docs.opengeospatial.org/is/17-003r2/17-003r2.html"/>
  </rdf:Property>
  
 
  
  <rdf:Property rdf:about="https://schema.org/processingDate">
    <schema:rangeIncludes rdf:resource="https://schema.org/DateTime"/>
    <schema:domainIncludes rdf:resource="https://schema.org/ProcessingInformation"/>
    <rdfs:label>processingDate</rdfs:label>
    <rdfs:comment>Processing date time.</rdfs:comment>
    <dcterms:source rdf:resource="http://docs.opengeospatial.org/is/17-003r2/17-003r2.html"/>
  </rdf:Property>
  
  
  <rdf:Property rdf:about="https://schema.org/processingLevel">
    <dcterms:source rdf:resource="http://docs.opengeospatial.org/is/17-003r2/17-003r2.html"/>
    <schema:rangeIncludes rdf:resource="https://schema.org/Text"/>
    <schema:domainIncludes rdf:resource="https://schema.org/ProcessingInformation"/>
    <rdfs:label>processingLevel</rdfs:label>
    <rdfs:comment>Processing level applied to the product: "1A", "1B", "1C", "2", "3".</rdfs:comment>
  </rdf:Property>
  
    
  <rdf:Property rdf:about="https://schema.org/processingMode">
    <schema:domainIncludes rdf:resource="https://schema.org/ProcessingInformation"/>
    <rdfs:comment>Processing mode taken from mission specific code list.
Examples of values are:
•	NRT
•	NOMINAL
•	BACKLOGGED
•	REPROCESSED
•	VALIDATE.</rdfs:comment>
    <dcterms:source rdf:resource="http://docs.opengeospatial.org/is/17-003r2/17-003r2.html"/>
    <schema:rangeIncludes rdf:resource="https://schema.org/Text"/>
    <rdfs:label>processingMode</rdfs:label>
  </rdf:Property>
      
 
  <rdf:Property rdf:about="https://schema.org/processorName">
    <rdfs:label>processorName</rdfs:label>
    <rdfs:comment>Processor software name (e.g. FastROSE).</rdfs:comment>
    <dcterms:source rdf:resource="http://docs.opengeospatial.org/is/17-003r2/17-003r2.html"/>
    <schema:domainIncludes rdf:resource="https://schema.org/ProcessingInformation"/>
    <schema:rangeIncludes rdf:resource="https://schema.org/Text"/>
  </rdf:Property>
  
  
   <!-- processorVersion --> 
  <rdf:Property rdf:about="https://schema.org/softwareVersion">
    <schema:domainIncludes rdf:resource="https://schema.org/ProcessingInformation"/>
   <!--  <owl:equivalentProperty rdf:resource="http://www.opengis.net/ont/eo-geojson/1.0/processorVersion"/>
    <dcterms:source rdf:resource="http://docs.opengeospatial.org/is/17-003r2/17-003r2.html"/>  -->
  </rdf:Property>
  
     
  <rdf:Property rdf:about="https://schema.org/productContentsType">
    <rdfs:label>productContentType</rdfs:label>
    <rdfs:comment>Classification of product according to ground type covered. Note cardinality allows for multiple instances of this property.
Allowed Values:
•	COASTAL
•	CONTINENTAL
•	HYDROLOGY
•	ICE
•	OPEN_OCEAN
•	OTHER
•	REGIONAL.</rdfs:comment>
    <schema:domainIncludes rdf:resource="https://schema.org/ProcessingInformation"/>
    <schema:rangeIncludes rdf:resource="https://schema.org/DefinedTerm"/>
    <dcterms:source rdf:resource="http://docs.opengeospatial.org/is/17-003r2/17-003r2.html"/>
  </rdf:Property>
  
  
  
    <!-- §7.7.3   CoverageDescription  -->
  
  <rdfs:Class rdf:about="https://schema.org/CoverageDescription">
    <rdfs:comment>Contains the properties related to the coverage. Its properties are inherited by the ProductInformation object.</rdfs:comment>
    <owl:equivalentClass rdf:resource="http://www.opengis.net/ont/eo-geojson/1.0/CoverageDescription"/>
    <dcterms:source rdf:resource="http://docs.opengeospatial.org/is/17-003r2/17-003r2.html"/>
    <rdfs:label>CoverageDescription</rdfs:label>
    <rdfs:subClassOf rdf:resource="https://schema.org/StructuredValue"/>
  </rdfs:Class>
  
  
  <rdf:Property rdf:about="https://schema.org/cloudCover">
    <schema:rangeIncludes rdf:resource="https://schema.org/Number"/>
    <rdfs:comment>Cloud cover percentage (i.e. uom=’%’).</rdfs:comment>
    <rdfs:label>cloudCover</rdfs:label>
    <dcterms:source rdf:resource="http://docs.opengeospatial.org/is/17-003r2/17-003r2.html"/>
    <schema:domainIncludes rdf:resource="https://schema.org/CoverageDescription"/>
  </rdf:Property>
  
    
  <rdf:Property rdf:about="https://schema.org/snowCover">
    <schema:rangeIncludes rdf:resource="https://schema.org/Number"/>
    <schema:domainIncludes rdf:resource="https://schema.org/CoverageDescription"/>
    <rdfs:comment>Snow cover percentage (i.e. uom=’%’).</rdfs:comment>
    <dcterms:source rdf:resource="http://docs.opengeospatial.org/is/17-003r2/17-003r2.html"/>
    <rdfs:label>snowCover</rdfs:label>
  </rdf:Property>
  

  
 
</rdf:RDF>